accountability

Protocols/ABC/Liveness.v
@@ -148,4 +148,265 @@ End Proof_of_Terminating_Convergence.
 
 End Terminating_Convergence.
 
+Module Accountability.
+
+Lemma conflicting_cert_quorum_in_proof rcerts v1 v2 nsigs1 nsigs2
+  (Hvneq : v1 <> v2)
+  (Hin1 : In (v1, nsigs1) rcerts)
+  (Hin2 : In (v2, nsigs2) rcerts) 
+  (Hcert_valid1 : certificate_valid v1 nsigs1)
+  (Hcert_valid2 : certificate_valid v2 nsigs2) :
+  incl (List.filter (fun n => In_dec Address_eqdec n (map fst nsigs1)) (map fst nsigs2)) 
+    (genproof rcerts).
+Proof.
+  hnf. intros nb' (Hin2' & Hin1'%sumbool_is_left)%filter_In.
+  pose proof Hin2' as Hin2''.
+  eapply valid_cert_sender_in in Hin1', Hin2'; eauto.
+  apply genproof_correct. 
+  now exists v1, v2, (sign v1 (key_map nb')), (sign v2 (key_map nb')), nsigs1, nsigs2.
+Qed.
+
+Definition nonbyz_confirmed n w : Prop := is_byz n = false /\ (localState w n).(conf).
+
+(* start *)
+Definition confirmed_different_values n1 n2 w : Prop :=
+  Eval unfold nonbyz_confirmed in
+  n1 <> n2 /\ nonbyz_confirmed n1 w /\ nonbyz_confirmed n2 w /\ 
+  (w @ n1).(submitted_value) <> (w @ n2).(submitted_value).
+
+Definition confirmed_different_values' n1 n2 w : Prop :=
+  Eval unfold nonbyz_confirmed in
+  n1 <> n2 /\ nonbyz_confirmed n1 w /\ nonbyz_confirmed n2 w /\ 
+  (w @ n1).(submitted_value) = Some (value_bft n1) /\
+  (w @ n2).(submitted_value) = Some (value_bft n2) /\
+  value_bft n1 <> value_bft n2.
+
+Fact confirmed_different_values_strengthen n1 n2 w (Hr : reachable w) :
+  confirmed_different_values n1 n2 w -> confirmed_different_values' n1 n2 w.
+Proof.
+  saturate.
+  intros (Hnneq & (H_n1_nonbyz & Hconf1) & (H_n2_nonbyz & Hconf2) & Hvneq).
+  pick confirmed_then_submitted as_ Hv1 by_ (pose proof (Hst n1) as []).
+  pick confirmed_then_submitted as_ Hv2 by_ (pose proof (Hst n2) as []).
+  saturate_assumptions. 
+  pick inv_submit_mixin as_ Hs1 by_ (pose proof (Hst n1) as []).
+  pick inv_submit_mixin as_ Hs2 by_ (pose proof (Hst n2) as []).
+  hnf.
+  destruct (submitted_value (w @ n1)) as [ v1 | ], (submitted_value (w @ n2)) as [ v2 | ]; try discriminate.
+  rewrite Hcoh in Hs1, Hs2. eqsolve.
+Qed.
+
+(* end; not represented as an explicit state *)
+Definition accountability w :=
+  exists byzs : list Address, 
+    NoDup byzs /\
+    N - (t0 + t0) <= length byzs /\
+    Forall is_byz byzs /\
+    (forall n, is_byz n = false -> incl byzs (genproof (w @ n).(received_certs))).
+
+Section Proof_of_Accountability.
+
+  Section Round1.
+
+  Variables (w : World) (n1 n2 : Address).
+  Hypothesis (H_w_reachable : reachable w) (Hstart : confirmed_different_values n1 n2 w).
+
+  Local Tactic Notation "prepare" hyp(H) :=
+    apply confirmed_different_values_strengthen in H; auto;
+    destruct H as (Hnneq & (Hnonbyz_n1 & Hconf1) & (Hnonbyz_n2 & Hconf2) & Hv1 & Hv2 & Hvneq); clear H.
+
+  (* well, using 4 packets instead of 2 is inevitable. *)
+  (* TODO self messaging is kind of weird *)
+  Definition mutual_lightcerts b1 b2 b3 b4 := Eval cbn in
+    let f src dst b := (mkP src dst (LightConfirmMsg 
+      (value_bft src, (lightsig_combine (localState w src).(collected_lightsigs)))) b) in
+    (f n1 n1 b1 :: f n1 n2 b2 :: f n2 n1 b3 :: f n2 n2 b4 :: nil). 
+
+  Definition pkts_needed_in_round_1 pkts :=
+    incl pkts (sentMsgs w) /\ Forall good_packet pkts /\
+    exists b1 b2 b3 b4, pkts = mutual_lightcerts b1 b2 b3 b4. 
+
+  Lemma round_1_pkts : exists pkts, pkts_needed_in_round_1 pkts.
+  Proof.
+    unfold pkts_needed_in_round_1, mutual_lightcerts. saturate. prepare Hstart.
+    pick inv_conf_lightconfmsg as_ Hc1 by_ (pose proof (Hl2h _ Hnonbyz_n1) as []).
+    pick inv_conf_lightconfmsg as_ Hc2 by_ (pose proof (Hl2h _ Hnonbyz_n2) as []).
+    pose proof (Hc1 _ Hv1 Hconf1 n1) as (b1 & Hin1).
+    pose proof (Hc1 _ Hv1 Hconf1 n2) as (b2 & Hin2).
+    pose proof (Hc2 _ Hv2 Hconf2 n1) as (b3 & Hin3).
+    pose proof (Hc2 _ Hv2 Hconf2 n2) as (b4 & Hin4).
+    rewrite Hcoh in Hin1, Hin2, Hin3, Hin4. eexists. split_and?. 
+    3: exists b1, b2, b3, b4; reflexivity.
+    - hnf. simpl. intuition (subst; auto).
+    - repeat constructor; auto.
+  Qed.
+
+  (* universally quantified *)
+  Variable (pkts : list Packet).
+  Hypotheses (Hround1 : pkts_needed_in_round_1 pkts).
+
+  Definition round_1_end w' :=
+    incl (mutual_lightcerts true true true true) (sentMsgs w').
+
+  Fact round_1_end_suffcond w' (Hincl : incl (map receive_pkt pkts) (sentMsgs w')) :
+    round_1_end w'.
+  Proof. hnf in Hround1. destruct Hround1 as (? & ? & (? & ? & ? & ? & ->)). auto. Qed.
+
+  (* at the same time as round 1 ends *)
+  Definition round_2_start w' :=
+    (* some conditions need to be kept *)
+    confirmed_different_values' n1 n2 w' /\
+    lightcert_conflict_check (w' @ n1).(received_lightcerts) /\
+    lightcert_conflict_check (w' @ n2).(received_lightcerts).
+
+  Lemma round_2_start_suffcond w0 l0 (Htrace0 : system_trace w l0) (Ew0 : w0 = final_world w l0) 
+    (Hw0 : round_1_end w0) : round_2_start w0.
+  Proof.
+    pose proof (reachable_by_trace Htrace0 H_w_reachable) as H_w0_reachable. rewrite <- Ew0 in H_w0_reachable.
+    (* clear H_w_reachable. *) saturate. prepare Hstart.
+
+    hnf in Hw0 |- *.
+    unfold mutual_lightcerts in Hw0. rewrite <- Forall_forall, !Forall_cons_iff in Hw0. 
+    destruct Hw0 as (H11 & H12 & H21 & H22 & _).
+    (* know that the combined lightsigs are good *)
+    (* TODO this is tedious! *)
+    (* FIXME: the proof may go too far. possibly using (w @ n) shoule be enough somewhere *)
+    apply persistent_invariants_trace in Htrace0; auto. 
+    pick inv_submit_mixin as_ Hs1 by_ (pose proof (Hst n1) as []).
+    pick inv_submit_mixin as_ Hs2 by_ (pose proof (Hst n2) as []).
+    pick inv_set_size as_ Hsz1 by_ (pose proof (Hst n1) as []).
+    pick inv_set_size as_ Hsz2 by_ (pose proof (Hst n2) as []).
+    pick inv_from_nodup as_ Hnodup1 by_ (pose proof (Hst n1) as []).
+    pick inv_from_nodup as_ Hnodup2 by_ (pose proof (Hst n2) as []).
+    pick inv_conf_correct as_ Hc1 by_ (pose proof (Hst n1) as []).
+    pick inv_conf_correct as_ Hc2 by_ (pose proof (Hst n2) as []).
+    pick submitted_value_persistent as_ Hvv1 by_ (pose proof (Htrace0 n1) as []).
+    pick submitted_value_persistent as_ Hvv2 by_ (pose proof (Htrace0 n2) as []).
+    pick conf_persistent as_ Hcc1 by_ (pose proof (Htrace0 n1) as []). 
+    pick conf_persistent as_ Hcc2 by_ (pose proof (Htrace0 n2) as []). 
+    pick conf_collected_lightsigs_persistent as_ Hls1 by_ (pose proof (Htrace0 n1) as []).
+    pick conf_collected_lightsigs_persistent as_ Hls2 by_ (pose proof (Htrace0 n2) as []). (* also these two *)
+    rewrite <- Ew0 in Hvv1, Hvv2, Hcc1, Hcc2, Hls1, Hls2. 
+    specialize (Hvv1 (value_bft n1)). specialize (Hvv2 (value_bft n2)). saturate_assumptions!.
+    rewrite Hvv1 in Hs1. rewrite Hcc1 in Hc1. rewrite Hvv2 in Hs2. rewrite Hcc2 in Hc2. rewrite Hls1 in *. rewrite Hls2 in *.
+    destruct Hs1 as (_ & Hs1 & _), Hs2 as (_ & Hs2 & _), Hsz1 as (Hsz1 & _), Hsz2 as (Hsz2 & _).
+    apply light_signatures_valid_for_combine in Hs1, Hs2; auto.
+    (* know that the lightcerts will not be rejected *)
+    let tac nn := assert (combined_verify (value_bft nn) (lightsig_combine (collected_lightsigs (w0 @ nn))))
+      by (apply combine_correct; exists (from_set (w0 @ nn)); split_and?; auto; try congruence)
+    in tac n1; tac n2.
+    let tac HH str := (let name := fresh "Hrcv" str in
+      pick inv_lightconfirmmsg_receive as_ name by_ (pose proof (Hh2l _ HH) as []))
+    in tac H11 ident:(_11); tac H12 ident:(_12); tac H21 ident:(_21); tac H22 ident:(_22).
+    saturate_assumptions!. 
+    rewrite !lightcert_conflict_check_correct. unfold confirmed_different_values'. split_and?; auto. 
+    all: exists (value_bft n1), (value_bft n2); do 2 eexists; split_and?; try eassumption; auto.
+  Qed.
+
+  End Round1.
+
+  Section Round2.
+
+  Variables (w : World) (n1 n2 : Address).
+  Hypothesis (H_w_reachable : reachable w) (Hstart : round_2_start n1 n2 w).
+
+  Local Tactic Notation "prepare" hyp(H) :=
+    destruct H as ((Hnneq & (Hnonbyz_n1 & Hconf1) & (Hnonbyz_n2 & Hconf2) & Hv1 & Hv2 & Hvneq) & Hcheck1 & Hcheck2); clear H.
+
+  Definition pkts_needed_in_round_2 pkts : Prop :=
+    pkts_needed 0 (* size does not matter here *) w (n1 :: n2 :: nil) pkts
+    (fun n => (ConfirmMsg (value_bft n, zip_from_sigs (w @ n)))) (fun _ _ => True). (* do not need extra predicate *)
+
+  Lemma round_2_pkts : exists pkts, pkts_needed_in_round_2 pkts.
+  Proof.
+    unfold pkts_needed_in_round_2. saturate. prepare Hstart.
+    exists (List.filter (fun p => 
+      match p.(msg) with
+      | ConfirmMsg _ =>
+        (negb (is_byz p.(src))) && (negb (is_byz p.(dst))) (* TODO maybe too general? *)
+      | _ => false
+      end) (sentMsgs w)).
+    hnf. split_and?; auto using incl_filter, le_0_n.
+    - repeat constructor; simpl; eqsolve. 
+    - apply Forall_forall. intros [ s d [] b ] (Hin & Hcheck)%filter_In; simpl in Hcheck; try discriminate.
+      now rewrite andb_true_iff, !negb_true_iff in Hcheck.
+    - intros n Hor. simpl in Hor.
+      apply and_wlog_r. 1: eqsolve. intros Hnonbyz_n. split; auto. intros nn Hnonbyz_nn.
+      (* know that n1 and n2 must have sent ConfirmMsg *)
+      pick inv_conf_confmsg as_ Hs1 by_ (pose proof (Hl2h _ Hnonbyz_n1) as []).
+      pick inv_conf_confmsg as_ Hs2 by_ (pose proof (Hl2h _ Hnonbyz_n2) as []).
+      specialize (Hs1 (value_bft n1)). specialize (Hs2 (value_bft n2)).
+      saturate_assumptions. rewrite Hcoh in Hs1, Hs2.
+      pose proof (Hs1 nn) as []. pose proof (Hs2 nn) as []. 
+      setoid_rewrite filter_In. simpl. rewrite Hnonbyz_n, Hnonbyz_nn. simpl.
+      destruct Hor as [ <- | [ <- | [] ] ]; eauto.
+  Qed.
+
+  (* universally quantified *)
+  Variable (pkts : list Packet).
+  Hypotheses (Hround2 : pkts_needed_in_round_2 pkts).
+
+  Definition round_2_end w' :=
+    forall n, is_byz n = false ->
+      In (mkP n1 n (ConfirmMsg (value_bft n1, zip_from_sigs (w @ n1))) true) (sentMsgs w') /\
+      In (mkP n2 n (ConfirmMsg (value_bft n2, zip_from_sigs (w @ n2))) true) (sentMsgs w').
+
+  Fact round_2_end_suffcond w' (Hincl : incl (map receive_pkt pkts) (sentMsgs w')) :
+    round_2_end w'.
+  Proof.
+    hnf in Hround2. pick ConfirmMsg as_ HH by_ (destruct_and? Hround2).
+    hnf. intros n Hnonbyz_n. split; apply Hincl.
+    1: specialize (HH n1 ltac:(simpl; tauto)).
+    2: specialize (HH n2 ltac:(simpl; tauto)).
+    all: destruct_and? HH; saturate_assumptions!.
+    all: destruct_exists; match goal with H : In _ pkts |- _ => apply (in_map receive_pkt) in H; now simpl in H end.
+  Qed.
+
+  Lemma accountability_suffcond w0 l0 (Htrace0 : system_trace w l0) (Ew0 : w0 = final_world w l0) 
+    (Hw0 : round_2_end w0) : accountability w0.
+  Proof.
+    saturate. 
+    pose proof (reachable_by_trace Htrace0 H_w_reachable) as H_w0_reachable. rewrite <- Ew0 in H_w0_reachable.
+    (* clear H_w_reachable. *) saturate. prepare Hstart.
+
+    hnf in Hw0.
+    (* TODO repeating *)
+    pick inv_submit_mixin as_ Hs1 by_ (pose proof (Hst n1) as []).
+    pick inv_submit_mixin as_ Hs2 by_ (pose proof (Hst n2) as []).
+    pick inv_set_size as_ Hsz1 by_ (pose proof (Hst n1) as []).
+    pick inv_set_size as_ Hsz2 by_ (pose proof (Hst n2) as []).
+    pick inv_from_nodup as_ Hnodup1 by_ (pose proof (Hst n1) as []).
+    pick inv_from_nodup as_ Hnodup2 by_ (pose proof (Hst n2) as []).
+    pick inv_conf_correct as_ Hc1 by_ (pose proof (Hst n1) as []).
+    pick inv_conf_correct as_ Hc2 by_ (pose proof (Hst n2) as []).
+    rewrite Hv1 in Hs1. rewrite Hconf1 in Hc1. rewrite Hv2 in Hs2. rewrite Hconf2 in Hc2. 
+    destruct Hs1 as (_ & _ & Hs1), Hs2 as (_ & _ & Hs2), Hsz1 as (_ & Hsz1), Hsz2 as (_ & Hsz2).
+    remember (List.filter (fun n' : Address => in_dec Address_eqdec n' (w @ n1).(from_set)) (w @ n2).(from_set)) as l eqn:El.
+    hnf. exists l. do 2 (try split_and).
+    - subst l. auto using NoDup_filter.
+    - subst l. apply quorum_intersection; auto; lia.
+    - apply and_wlog_l.
+      + intros HH. apply Forall_forall. intros x Hin.
+        (* exploit that there exists some non-Byz node *)
+        specialize (HH _ Hnonbyz_n1). eapply HH, genproof_soundness_always_holds in Hin; auto.
+      + intros n Hnonbyz_n. specialize (Hw0 _ Hnonbyz_n). destruct Hw0 as (Hq1 & Hq2). 
+        (* need to show that they will be received *)
+        pick inv_confirmmsg_receive as_ Hr1 by_ (pose proof (Hh2l0 _ Hq1) as []).
+        pick inv_confirmmsg_receive as_ Hr2 by_ (pose proof (Hh2l0 _ Hq2) as []).
+        saturate_assumptions.
+        unfold zip_from_sigs in Hr1, Hr2. rewrite combine_length in Hr1, Hr2. rewrite <- Hsz1, -> Hc1 in Hr1. rewrite <- Hsz2, -> Hc2 in Hr2.
+        specialize (Hr1 (NoDup_combine_l _ _ Hnodup1) ltac:(lia)).
+        specialize (Hr2 (NoDup_combine_l _ _ Hnodup2) ltac:(lia)).
+        subst l.
+        rewrite <- (combine_map_fst (from_set (w @ n1)) (collected_sigs (w @ n1))) by auto.
+        rewrite <- (combine_map_fst (from_set (w @ n2)) (collected_sigs (w @ n2))) by auto.
+        eapply conflicting_cert_quorum_in_proof; try hypothesis. 
+  Qed.
+
+  End Round2.
+
+End Proof_of_Accountability.
+
+End Accountability.
+
 End ACLiveness.
