Protocols/ABC/Liveness_tla.v
@@ -19,6 +19,7 @@ Include Liveness A M BTh BSett P0 PSOp ACP Ns ACAdv ACN.
 (* empirical, but maybe useful? *)
 Local Ltac aux Htmp :=
   match type of Htmp with
+  (* the packets must be at the outmost level *)
   | (exists (_ : list ?t), _) =>
     tryif convert t Packet
     then 
@@ -50,6 +51,23 @@ Lemma terminating_convergence_in_tla v (H_byz_minor : num_byz ≤ t0) :
   ⌜ all_honest_nodes_submitted v ⌝ ~~> ⌜ all_honest_nodes_confirmed v ⌝.
 Proof.
   delivering round_1_pkts which ends at round_1_end_suffcond is sufficient because all_honest_nodes_confirmed_suffcond.
+Qed.
+
+End A.
+
+Section A.
+
+Import Accountability.
+
+Lemma accountability_in_tla :
+  ⌜ init ⌝ ∧ □ ⟨ next ⟩ ∧ fairness ⊢
+  ⌜ λ w, ∃ n1 : Address, ∃ n2 : Address, confirmed_different_values n1 n2 w ⌝ ~~> ⌜ accountability ⌝.
+Proof.
+  (* intro first *)
+  let tac n := rewrite <- exist_state_pred; apply leads_to_exist_intro; intros n in tac n1; tac n2.
+  tla_apply (leads_to_trans _ (⌜ round_2_start n1 n2 ⌝)). tla_split.
+  - delivering round_1_pkts which ends at round_1_end_suffcond is sufficient because round_2_start_suffcond.
+  - delivering round_2_pkts which ends at round_2_end_suffcond is sufficient because accountability_suffcond.
 Qed.
 
 End A.
